Change mem to an inductive type

src/AsyncDisk.v
@@ -162,23 +162,23 @@ Qed.
 
 
 Definition sync_mem AT AEQ (m : @mem AT AEQ valuset) : @mem AT AEQ valuset :=
-  fun a => match m a with
-    | None => None
-    | Some (v, _) => Some (v, nil)
-    end.
+  M (fun a => match m a with
+        | None => None
+        | Some (v, _) => Some (v, nil)
+        end).
 
 Definition sync_addr AT AEQ (m : @mem AT AEQ valuset) a : @mem AT AEQ valuset :=
-  fun a' => if AEQ a a' then
-    match m a with
-    | None => None
-    | Some (v, _) => Some (v, nil)
-    end else m a'.
+  M (fun a' => if AEQ a a' then
+              match m a with
+              | None => None
+              | Some (v, _) => Some (v, nil)
+              end else m a').
 
 Lemma sync_addr_ne : forall AT AEQ (m : @mem AT AEQ valuset) a a',
   a <> a' ->
   (sync_addr m a) a' = m a'.
 Proof.
-  unfold sync_addr; intros.
+  unfold sync_addr; intros; simpl.
   destruct (AEQ a a'); try congruence.
 Qed.
 
@@ -187,7 +187,7 @@ Lemma sync_addr_eq : forall AT AEQ (m : @mem AT AEQ valuset) a a' vs,
   m a' = Some vs ->
   (sync_addr m a) a' = Some (fst vs, nil).
 Proof.
-  unfold sync_addr; intros; subst.
+  unfold sync_addr; intros; subst; simpl.
   destruct (AEQ a' a'); try congruence.
   destruct (m a'); try congruence.
   inversion H0; subst.
