src/Mem.v
@@ -6,8 +6,14 @@ Definition EqDec (T : Type) := forall (a b : T), {a = b} + {a <> b}.
 
 (* generalized memory of any address / value type *)
 
-Definition mem {A : Type} {AEQ : EqDec A} {V : Type} := A -> option V.
-Definition empty_mem {A : Type} {AEQ : EqDec A} {V : Type} : @mem A AEQ V := fun a => None.
+Record mem {A : Type} {AEQ : EqDec A} {V : Type} :=
+  M { memory : A -> option V; }.
+
+Arguments M {A AEQ V}.
+
+Coercion memory : mem >-> Funclass.
+
+Definition empty_mem {A : Type} {AEQ : EqDec A} {V : Type} : @mem A AEQ V := M (fun a => None).
 
 Section GenMem.
   Variable A : Type.
@@ -15,180 +21,161 @@ Section GenMem.
   Variable AEQ : EqDec A.
 
   Definition upd (m : @mem A AEQ V) (a : A) (v : V) : @mem A AEQ V :=
-    fun a' => if AEQ a' a then Some v else m a'.
+    M (fun a' => if AEQ a' a then Some v else m a').
 
   Definition updSome (m : @mem A AEQ V) (a : A) (v : V) : @mem A AEQ V :=
-    fun a' => if AEQ a' a then
-      match m a with
-      | None => None
-      | Some _ => Some v
-      end else m a'.
+    M (fun a' => if AEQ a' a then
+                match m a with
+                | None => None
+                | Some _ => Some v
+                end else m a').
 
   Definition delete (m : @mem A AEQ V) (a : A) : @mem A AEQ V :=
-    fun a' => if AEQ a' a then None else m a'.
+    M (fun a' => if AEQ a' a then None else m a').
 
   Definition insert (m : @mem A AEQ V) (a : A) (v : V) : @mem A AEQ V :=
-    fun a' => if AEQ a' a then
+    M (fun a' => if AEQ a' a then
       match m a with
       | None => Some v
       | Some _ => m a'
-      end else m a'.
+      end else m a').
+
+  Ltac t :=
+    intros; subst; unfold upd, updSome, insert, delete; simpl;
+    repeat match goal with
+           | [ m: mem |- _ ] =>
+             destruct m; simpl in *
+           | [ |- context[if AEQ ?a ?a' then _ else _] ] =>
+             destruct (AEQ a a')
+           | [ |- context[match ?d with _ => _ end] ] =>
+             destruct d eqn:?
+           | [ |- _ = _ :> mem ] =>
+             apply f_equal
+           | [ |- _ = _ :> (_ -> _) ] =>
+             apply functional_extensionality
+           | _ => progress intros
+           | _ => congruence
+           | _ => tauto
+           end.
+
+  Implicit Type (m:@mem A AEQ V).
 
   Theorem upd_eq : forall m (a : A) (v : V) a',
     a' = a -> upd m a v a' = Some v.
   Proof.
-    intros; subst; unfold upd.
-    destruct (AEQ a a); tauto.
+    t.
   Qed.
 
   Theorem updSome_eq : forall m (a : A) (v v' : V) a',
-    m a = Some v' -> a' = a -> updSome m a v a' = Some v.
+      m a = Some v' -> a' = a ->
+      updSome m a v a' = Some v.
   Proof.
-    intros; subst; unfold updSome.
-    rewrite H.
-    destruct (AEQ a a); tauto.
+    t.
   Qed.
 
   Theorem insert_eq : forall m (a : A) (v v' : V) a',
     m a = None -> a' = a -> insert m a v a' = Some v.
   Proof.
-    intros; subst; unfold insert.
-    rewrite H.
-    destruct (AEQ a a); congruence.
+    t.
   Qed.
 
   Theorem upd_ne : forall m (a : A) (v : V) a',
     a' <> a -> upd m a v a' = m a'.
   Proof.
-    intros; subst; unfold upd.
-    destruct (AEQ a' a); tauto.
+    t.
   Qed.
 
   Theorem updSome_ne : forall m (a : A) (v : V) a',
     a' <> a -> updSome m a v a' = m a'.
   Proof.
-    intros; subst; unfold updSome.
-    destruct (AEQ a' a); tauto.
+    t.
   Qed.
 
   Theorem insert_ne : forall m (a : A) (v : V) a',
     a' <> a -> insert m a v a' = m a'.
   Proof.
-    intros; subst; unfold insert.
-    destruct (AEQ a' a); congruence.
+    t.
   Qed.
 
   Theorem upd_repeat: forall m (a : A) (v v':V),
     upd (upd m a v') a v = upd m a v.
   Proof.
-    intros; apply functional_extensionality; unfold upd; intros.
-    destruct (AEQ a a); try congruence.
-    destruct (AEQ x a); auto.
+    t.
   Qed.
 
   Theorem updSome_repeat: forall m (a : A) (v v':V),
     updSome (updSome m a v') a v = updSome m a v.
   Proof.
-    intros; apply functional_extensionality; unfold updSome; intros.
-    destruct (AEQ a a); try congruence.
-    destruct (AEQ x a); auto.
-    destruct (m a); auto.
+    t.
   Qed.
 
   Theorem insert_repeat: forall m (a : A) (v v':V),
     insert (insert m a v) a v' = insert m a v.
   Proof.
-    intros; apply functional_extensionality; unfold insert at 1; intros.
-    destruct (AEQ a a); try congruence.
-    destruct (AEQ x a); auto.
-    subst. unfold insert; simpl.
-    destruct (AEQ a a); try congruence.
-    destruct (m a); auto.
+    t.
   Qed.
 
   Theorem upd_nop: forall m (a : A) (v : V),
     m a = Some v ->
     upd m a v = m.
   Proof.
-    intros; apply functional_extensionality; intros.
-    case_eq (AEQ a x); intros; subst.
-    repeat erewrite upd_eq; eauto.
-    repeat rewrite upd_ne; auto.
+    t.
   Qed.
 
   Theorem updSome_nop: forall m (a : A) (v : V),
     m a = Some v ->
     updSome m a v = m.
   Proof.
-    intros; apply functional_extensionality; intros.
-    case_eq (AEQ a x); intros; subst.
-    repeat erewrite updSome_eq; eauto.
-    repeat rewrite updSome_ne; auto.
+    t.
   Qed.
 
   Theorem updSome_none : forall m (a : A) (v : V),
     m a = None ->
     updSome m a v = m.
   Proof.
-    unfold updSome; intros; apply functional_extensionality; intros.
-    rewrite H.
-    destruct (AEQ x a); subst; auto.
+    t.
   Qed.
 
   Theorem upd_comm: forall m (a0 : A) (v0 : V) a1 v1, a0 <> a1
     -> upd (upd m a0 v0) a1 v1 = upd (upd m a1 v1) a0 v0.
   Proof.
-    intros; apply functional_extensionality; unfold upd; intros.
-    destruct (AEQ a1 a0); destruct (AEQ a0 a1); try congruence.
-    case_eq (AEQ x a1); case_eq (AEQ x a0); intros; subst; try congruence.
+    t.
   Qed.
 
   Theorem updSome_comm: forall m (a0 : A) (v0 : V) a1 v1, a0 <> a1
     -> updSome (updSome m a0 v0) a1 v1 = updSome (updSome m a1 v1) a0 v0.
   Proof.
-    intros; apply functional_extensionality; unfold updSome; intros.
-    destruct (AEQ a1 a0); destruct (AEQ a0 a1); try congruence.
-    case_eq (AEQ x a1); case_eq (AEQ x a0); intros; subst; try congruence.
+    t.
   Qed.
 
   Theorem updSome_insert_comm: forall m (a0 : A) (v0 : V) a1 v1, a0 <> a1
     -> updSome (insert m a0 v0) a1 v1 = insert (updSome m a1 v1) a0 v0.
   Proof.
-    intros; apply functional_extensionality; unfold updSome, insert; intros.
-    destruct (AEQ a1 a0); destruct (AEQ a0 a1); try congruence.
-    case_eq (AEQ x a1); case_eq (AEQ x a0); intros; subst; try congruence.
+    t.
   Qed.
 
   Theorem updSome_delete_comm: forall m (a0 : A) a1 (v1 : V), a0 <> a1
     -> updSome (delete m a0) a1 v1 = delete (updSome m a1 v1) a0.
   Proof.
-    intros; apply functional_extensionality; unfold updSome, delete; intros.
-    destruct (AEQ a1 a0); destruct (AEQ a0 a1); try congruence.
-    case_eq (AEQ x a1); case_eq (AEQ x a0); intros; subst; try congruence.
+    t.
   Qed.
 
   Theorem insert_comm: forall m (a0 : A) (v0 : V) a1 v1, a0 <> a1
     -> insert (insert m a0 v0) a1 v1 = insert (insert m a1 v1) a0 v0.
   Proof.
-    intros; apply functional_extensionality; unfold insert; intros.
-    destruct (AEQ a1 a0); destruct (AEQ a0 a1); try congruence.
-    case_eq (AEQ x a1); case_eq (AEQ x a0); intros; subst; try congruence.
+    t.
   Qed.
 
   Theorem insert_delete_comm: forall m (a0 : A) a1 (v1 : V), a0 <> a1
     -> insert (delete m a0) a1 v1 = delete (insert m a1 v1) a0.
   Proof.
-    intros; apply functional_extensionality; unfold insert, delete; intros.
-    destruct (AEQ a1 a0); destruct (AEQ a0 a1); try congruence.
-    case_eq (AEQ x a1); case_eq (AEQ x a0); intros; subst; try congruence.
+    t.
   Qed.
 
   Theorem delete_comm: forall m (a0 : A) a1, a0 <> a1
     -> delete (delete m a0) a1 = delete (delete m a1) a0.
   Proof.
-    intros; apply functional_extensionality; unfold delete; intros.
-    destruct (AEQ a1 a0); destruct (AEQ a0 a1); try congruence.
-    case_eq (AEQ x a1); case_eq (AEQ x a0); intros; subst; try congruence.
+    t.
   Qed.
 
 End GenMem.
